

**Q1. 22 January Shift 1**

If  $\int (\sin x)^{\frac{-11}{2}} (\cos x)^{\frac{-5}{2}} dx = -\frac{p_1}{q_1} (\cot x)^{\frac{9}{2}} - \frac{p_2}{q_2} (\cot x)^{\frac{5}{2}} - \frac{p_3}{q_3} (\cot x)^{\frac{1}{2}} + \frac{p_4}{q_4} (\cot x)^{\frac{-3}{2}} + C$ , where  $p_i$  and  $q_i$  are positive integers with  $\gcd(p_i, q_i) = 1$  for  $i = 1, 2, 3, 4$  and  $C$  is the constant of integration, then  $\frac{15p_1p_2p_3p_4}{q_1q_2q_3q_4}$  is equal to

**Q2. 23 January Shift 1**

Let  $f(x) = \int \frac{(2-x^2) \cdot e^x}{(\sqrt{1+x})(1-x)^{3/2}} dx$ . If  $f(0) = 0$ , then  $f\left(\frac{1}{2}\right)$  is equal to:

- (1)  $\sqrt{3e} - 1$  (2)  $\sqrt{3e} + 1$  (3)  $\sqrt{2e} + 1$  (4)  $\sqrt{2e} - 1$

**Q3. 23 January Shift 2**

Let  $I(x) = \int \frac{3dx}{(4x+6)(\sqrt{4x^2+8x+3})}$  and  $I(0) = \frac{\sqrt{3}}{4} + 20$ . If  $I\left(\frac{1}{2}\right) = \frac{a\sqrt{2}}{b} + c$ , where  $a, b, c \in \mathbb{N}$ ,  $\gcd(a, b) = 1$ , then

$a + b + c$  is equal to

- (1) 30 (2) 31 (3) 29 (4) 28

**Q4. 24 January Shift 1**

Let  $f(t) = \int \left( \frac{1 - \sin(\log_e t)}{1 - \cos(\log_e t)} \right) dt, t > 1$ .

If  $f(e^{\pi/2}) = -e^{\pi/2}$  and  $f(e^{\pi/4}) = \alpha e^{\pi/4}$ , then  $\alpha$  equals

- (1)  $1 + \sqrt{2}$  (2)  $-1 - \sqrt{2}$  (3)  $-1 - 2\sqrt{2}$  (4)  $-1 + \sqrt{2}$

**Q5. 28 January Shift 2**

Let  $f(x) = \int \frac{dx}{x^{\left(\frac{2}{3}\right)+2x^{\left(\frac{1}{2}\right)}}$  be such that  $f(0) = -26 + 24 \log_e(2)$ . If  $f(1) = a + b \log_e(3)$ , where  $a, b \in \mathbb{Z}$ , then  $a + b$  is equal to :

- (1) -26 (2) -11 (3) -5 (4) -18

**ANSWER KEYS**

1. 16 2. (1) 3. (2) 4. (2) 5. (2)